src/Std/Tactic/BVDecide/Bitblast/BVExpr/Circuit/Lemmas/Operations/Cpop.lean
@@ -10,6 +10,7 @@ public import Std.Tactic.BVDecide.Bitblast.BVExpr.Circuit.Lemmas.Basic
 public import Std.Tactic.BVDecide.Bitblast.BVExpr.Circuit.Impl.Operations.Cpop
 public import Std.Tactic.BVDecide.Bitblast.BVExpr.Circuit.Lemmas.Const
 public import Std.Tactic.BVDecide.Bitblast.BVExpr.Circuit.Lemmas.Operations.Sub
+public import Std.Tactic.BVDecide.Bitblast.BVExpr.Circuit.Lemmas.Operations.Append
 public import Std.Tactic.BVDecide.Bitblast.BVExpr.Circuit.Lemmas.Operations.Eq
 public import Std.Tactic.BVDecide.Bitblast.BVExpr.Circuit.Lemmas.Operations.ZeroExtend
 public import Std.Tactic.BVDecide.Bitblast.BVExpr.Circuit.Lemmas.Operations.Extract
@@ -218,6 +219,7 @@ theorem denote_blastAddVec
   (hold' : 2 * (iter_num - 1) < old_length)
   (old_layer_bv : BitVec (old_length * w))
   (hval : 0 < l_length)
+  (hw : 0 < w)
   -- the bits added already denote to the corresponding entry in acc
   (hold : ∀ (idx : Nat) (hidx : idx < old_length * w),
           ⟦aig, old_layer.get idx hidx, assign⟧ = old_layer_bv.getLsbD idx)
@@ -237,105 +239,115 @@ theorem denote_blastAddVec
   split at hgen
   · case _ hgen' =>
     rw [← hgen]
-    expose_names
     rw [denote_blastAddVec]
     · omega
+    · omega
     · intros idx hidx
-      specialize hold idx hidx
-      rw [AIG.LawfulVecOperator.denote_mem_prefix (f := blastAdd)]
-      rw [AIG.LawfulVecOperator.denote_mem_prefix (f := blastExtract)]
-      · simp [hold]
+      rw [AIG.LawfulVecOperator.denote_mem_prefix]
+      · rw [AIG.LawfulVecOperator.denote_mem_prefix]
+        · rw [AIG.LawfulVecOperator.denote_mem_prefix]
+          · rw [AIG.LawfulVecOperator.denote_mem_prefix]
+            · simp [hold]
+            · simp [Ref.hgate]
+          · simp
+            exact (old_layer.get idx hidx).hgate
+        · simp
+          exact (old_layer.get idx hidx).hgate
       · simp
+        apply LawfulVecOperator.lt_size_of_lt_aig_size
         exact (old_layer.get idx hidx).hgate
-      · simp
-        exact (old_layer.get idx hidx).hgate
-    · intros idx hidx
-      expose_names
-      let res := (blastAdd (blastExtract aig { w := old_length * w, vec := old_layer, start := 2 * iter_num * w }).aig
-                  { lhs := (blastExtract aig { w := old_length * w, vec := old_layer, start := 2 * iter_num * w }).vec,
-                    rhs := (if 2 * iter_num + 1 < old_length then (blastExtract aig
-                                { w := old_length * w, vec := old_layer, start := (2 * iter_num + 1) * w }).vec
-                              else blastConst aig 0#w).cast (by apply LawfulVecOperator.le_size (f := blastExtract))})
-      have hres : res = (blastAdd (blastExtract aig { w := old_length * w, vec := old_layer, start := 2 * iter_num * w }).aig
-                  {lhs := (blastExtract aig { w := old_length * w, vec := old_layer, start := 2 * iter_num * w }).vec,
-                    rhs := (if 2 * iter_num + 1 < old_length then (blastExtract aig
-                                { w := old_length * w, vec := old_layer, start := (2 * iter_num + 1) * w }).vec
-                              else blastConst aig 0#w).cast (by apply LawfulVecOperator.le_size (f := blastExtract))}) := rfl
-      have h1 : 2 * iter_num / 2 * w + w = (2 * iter_num + 2) / 2 * w := by
-          rw [show 2 * iter_num / 2 * w + w = 2 * iter_num / 2 * w + 1 * w by omega]
-          rw [← Nat.add_mul]
-          simp
-      let elem := (blastAdd (blastExtract aig { w := old_length * w, vec := old_layer, start := 2 * iter_num * w }).aig
-          { lhs := (blastExtract aig { w := old_length * w, vec := old_layer, start := 2 * iter_num * w }).vec,
-            rhs :=
-              (if 2 * iter_num + 1 < old_length then
-                    (blastExtract aig
-                        { w := old_length * w, vec := old_layer, start := (2 * iter_num + 1) * w }).vec
-                  else blastConst aig 0#w).cast (by apply LawfulVecOperator.le_size (f := blastExtract))})
-      simp
-
-      have hc1 : w + iter_num * w = (iter_num + 1) * w := by simp [Nat.add_mul]; omega
-      have hc2 : (iter_num + 1) * w = w + iter_num * w := by simp [Nat.add_mul]; omega
-      have hc3 : w + iter_num * w = (iter_num + 1) * w := by simp [Nat.add_mul]; omega
-      have : (hc1▸
-                hc2 ▸
-                  hc3 ▸
-                    (blastAdd (blastExtract aig { w := old_length * w, vec := old_layer, start := 2 * iter_num * w }).aig
-                            {
-                              lhs :=
-                                (blastExtract aig
-                                    { w := old_length * w, vec := old_layer, start := 2 * iter_num * w }).vec,
-                              rhs :=
-                                (if 2 * iter_num + 1 < old_length then
-                                      (blastExtract aig
-                                          { w := old_length * w, vec := old_layer, start := (2 * iter_num + 1) * w }).vec
-                                    else blastConst aig 0#w).cast
-                                  (by apply LawfulVecOperator.le_size) }).vec.append
-                    (new_layer.cast (by apply LawfulVecOperator.le_size))).get idx hidx
-          = ((blastAdd (blastExtract aig { w := old_length * w, vec := old_layer, start := 2 * iter_num * w }).aig
-                            {
-                              lhs :=
-                                (blastExtract aig
-                                    { w := old_length * w, vec := old_layer, start := 2 * iter_num * w }).vec,
-                              rhs :=
-                                (if 2 * iter_num + 1 < old_length then
-                                      (blastExtract aig
-                                          { w := old_length * w, vec := old_layer, start := (2 * iter_num + 1) * w }).vec
-                                    else blastConst aig 0#w).cast
-                                  (by apply LawfulVecOperator.le_size) }).vec.append
-                    (new_layer.cast (by apply LawfulVecOperator.le_size))).get idx (by
-                    omega) := by
-                  congr
-                  ·
-
-                    sorry
-                  · exact heq_of_eqRec_eq (congrArg (LT.lt idx) hc2) rfl
-      rw [this]
-      let bvRes:= BitVec.pps_layer 0 old_layer_bv 0#(0 * w) (by omega) (by omega)
-
-      sorry
+    · intros idx2 hidx2
+      simp [denote_blastAppend]
+      split
+      · case _ hsplit =>
+        rw [AIG.LawfulVecOperator.denote_mem_prefix]
+        · rw [AIG.LawfulVecOperator.denote_mem_prefix]
+          · rw [AIG.LawfulVecOperator.denote_mem_prefix]
+            · rw [hnew]
+            · simp [Ref.hgate]
+          · exact (new_layer.get idx2 (Eq.mpr_prop (Eq.refl (idx2 < iter_num * w)) hsplit)).hgate
+        · exact (new_layer.get idx2 (Eq.mpr_prop (Eq.refl (idx2 < iter_num * w)) hsplit)).hgate
+      · case _ hsplit1 =>
+        have ⟨bvRes, bvRes_proof⟩ := BitVec.pps_layer 0 old_layer_bv 0#(0 * w) (by omega) (by omega)
+        simp
+        have bvRes_proof' := bvRes_proof iter_num (by omega) (by omega)
+        let lhs_bv := BitVec.extractLsb' (2 * iter_num * w) w old_layer_bv
+        let rhs_bv := if h : 2 * iter_num + 1 < old_length
+                      then BitVec.extractLsb' ((2 * iter_num + 1) * w) w old_layer_bv else 0
+        rw [denote_blastAdd (rhs := rhs_bv) (lhs := lhs_bv)]
+        · -- have : ∀ k,  (BitVec.extractLsb' (iter_num * w) w bvRes).getLsbD k =
+          let k := idx2 - iter_num * w
+          have hksum : idx2 = iter_num * w + k := by omega
+          rw [hksum]
+          rw [show iter_num * w + k - iter_num * w = k by omega]
+          specialize bvRes_proof (i := iter_num) (by omega) (by omega)
+          have hlsbd := BitVec.getLsbD_extractLsb' (x := bvRes) (start := iter_num * w) (len := w) (i := k)
+          have : k < w := by
+            apply Classical.byContradiction
+            intros hcontra
+            simp [hksum, Nat.add_mul] at hidx2
+            omega
+          simp only [this, decide_true, Bool.true_and] at hlsbd
+          simp only [dite_eq_ite, BitVec.ofNat_eq_ofNat, lhs_bv, rhs_bv]
+          rw [← hlsbd]
+          simp [bvRes_proof]
+        · intros idx hidx
+          simp only [BitVec.getLsbD_extractLsb', lhs_bv]
+          have := BitVec.getLsbD_extractLsb' (x := old_layer_bv) (start := 2 * iter_num * w) (len := w) (i := idx)
+          rw [← this]
+          rw [AIG.LawfulVecOperator.denote_mem_prefix]
+          · simp
+            rw [denote_blastExtract]
+            split
+            · simp [hidx, hold]
+            · case _ hh =>
+              simp at hh
+              simp [hh]
+          · exact
+            (((blastExtract aig
+                          { w := old_length * w, vec := old_layer,
+                            start := 2 * iter_num * w }).vec.cast
+                    (blastAddVec._proof_10 aig iter_num old_layer
+                      (blastAddVec._proof_9 aig iter_num old_layer))).get
+                idx hidx).hgate
+        · intros idx1 hidx1
+          simp only [dite_eq_ite, BitVec.ofNat_eq_ofNat, rhs_bv]
+          have :
+            ((if 2 * iter_num + 1 < old_length then BitVec.extractLsb' ((2 * iter_num + 1) * w) w old_layer_bv else 0#w).getLsbD idx1) =
+            ((decide (idx1 < w) && old_layer_bv.getLsbD ((2 * iter_num + 1) * w + idx1))) := by
+            simp [hidx1]
+            split
+            · case _ hh =>
+              simp
+            · case _ hh =>
+              simp at hh
+              have h1 : old_length * w ≤ (2 * iter_num + 1) * w := by
+                exact Nat.mul_le_mul_right w hh
+              have h2 : old_length * w ≤ (2 * iter_num) * w + w := by
+                simp [Nat.add_mul] at h1; omega
+              have h3 : old_length * w ≤ (2 * iter_num + 1) * w + idx1 := by
+                omega
+              simp [h3]
+          rw [this]
+          have := BitVec.getLsbD_extractLsb' (x := old_layer_bv) (start := (2 * iter_num + 1) * w) (len := w) (i := idx1)
+          rw [← this]
+          rw [denote_blastExtract]
+          split
+          · simp
+            rw [AIG.LawfulVecOperator.denote_mem_prefix]
+            · simp [hold, hidx1]
+            · (expose_names; exact (old_layer.get ((2 * iter_num + 1) * w + idx1) h).hgate)
+          · case _ hh =>
+            simp at hh
+            simp
+            have h3 : old_length * w ≤ (2 * iter_num + 1) * w + idx1 := by
+              omega
+            simp [h3]
   · case _ hgen' =>
-    rw [← hgen]
-    have hcast : iter_num = (old_length + 1) / 2 := by
-      omega
-    have hcast1 : idx < iter_num * w := by
-      rw [← hcast] at hidx
-      exact hidx
-    have : (hcast▸new_layer).get idx (by omega) = new_layer.get idx (by omega) := by
-      congr
-      · omega
-      · apply eqRec_heq
-      · exact
-        heq_of_eqRec_eq
-          (congrArg (LT.lt idx) (congrFun (congrArg HMul.hMul (id (Eq.symm hcast))) w)) rfl
-    conv =>
-      lhs
-      arg 2
-      arg 2
-      simp
-    simp [this]
-    specialize hnew idx (by omega)
-    simp [hnew]
+    have h : iter_num = (old_length + 1) / 2 := by omega
+    subst h
+    rw [← hgen, hnew]
+
 
 theorem pss_eq_of_eq (x y : BitVec (l_length * w)) (hxy : x = y)
   (xproof : x.addRecAux l_length 0#w = kx)
@@ -444,6 +456,7 @@ theorem denote_go
     · intros idx hidx
       rw [denote_blastAddVec (old_layer_bv := l_bv) (l_length := l_length)]
       · omega
+      · omega
       · intros idx hidx
         apply hpar
       · intros idx hidx
@@ -463,8 +476,6 @@ theorem denote_go
     rw [hcasteq]
     simp [hpar]
 
-
-
 @[simp]
 theorem denote_blastCpop (aig : AIG α) (xc : RefVec aig w) (x : BitVec w) (assign : α → Bool)
       (hx : ∀ (idx : Nat) (hidx : idx < w), ⟦aig, xc.get idx hidx, assign⟧ = x.getLsbD idx)
@@ -475,11 +486,11 @@ theorem denote_blastCpop (aig : AIG α) (xc : RefVec aig w) (x : BitVec w) (assi
     generalize hgen : blastCpop aig xc = res
     unfold blastCpop at hgen
     rw [BitVec.cpop_eq_pps]
-
     split at hgen
     · intros idx hidx
       rw [← hgen]
-      simp
+      simp only [BitVec.ofNat_eq_ofNat, Lean.Elab.WF.paramLet, BitVec.addRecAux_succ,
+        BitVec.addRecAux_zero]
       rw [denote_go (l_bv := BitVec.extractAndExtendPopulate w x)]
       · simp [show ¬ w = 0 by omega]
       · omega
